further simplified consensus checks. fixed resLe to not relate delegated and undelegated cases as in the usecases, that part will remain the same: consensus checks will have the exact same view as execution. but just now realized that may not work as in execution, it can be undelegated while it can be delegated in consensus

monadproofs/proofs/reservebal.v
@@ -183,7 +183,7 @@ Definition isAllowedToEmpty
  TODO: tell coqdoc to print Set as Type*)
 Record NotDelCaseExecRes  : Set := mkNotDelCase
   {
-    balanceLb: N;
+    balanceLb: Z;
     configuredRB: N;
     feeSolvent: bool (* sometimes,  *)
   }.
@@ -252,39 +252,45 @@ TODO: move updateKey preTxResBalances addr to the top
 Notation delegated := inl.
 Notation notdelegated := inr.
 (* TODO: rename to shallowExecTx *)
-Definition remainingEffReserveBals (preCandidateTxRes: EffReserveBals) (intermediates: list TxWithHdr) (candidateTx: TxWithHdr)
-  : EffReserveBals :=
+Open Scope Z_scope.
+Definition remainingEffReserveBals (preCandidateTxRes: EffReserveBals) (candidateTx: TxWithHdr)
+  : EffReserveBals := fun addr =>
   let maxTxFee := maxTxFee candidateTx in
-  fun addr =>
-    match preCandidateTxRes addr with
-    | delegated erb => delegated(
-        if bool_decide (sender candidateTx <> addr)
-        then erb
-        else
-          match reserveBalUpdateOfTx candidateTx with
-          | Some newRb =>
-              (erb - maxTxFee) `min` newRb
-          | None => (erb - maxTxFee)
-          end)
-    | notdelegated {| balanceLb := balLb; configuredRB := crb; feeSolvent := fs|} =>
-        if bool_decide (addr ∈ dels candidateTx.1.2)
-        then delegated ((balLb - maxTxFee) `min` crb)
-        else if bool_decide (sender candidateTx <> addr)
-             then preCandidateTxRes addr
-             else notdelegated
-                    {| balanceLb := balLb - value candidateTx - maxTxFee;
-                      configuredRB := crb;
-                      feeSolvent := fs && bool_decide (maxTxFee <= balLb)|}
-    end.
+  match preCandidateTxRes addr with
+  | delegated erb =>
+      delegated(
+          if bool_decide (sender candidateTx <> addr)
+          then erb
+          else
+            match reserveBalUpdateOfTx candidateTx with
+            | Some newRb =>
+                (erb - maxTxFee) `min` newRb
+            | None => (erb - maxTxFee)
+            end)
+  | notdelegated sres =>
+      if bool_decide (addr ∈ dels candidateTx.1.2)
+      then delegated
+            ((if bool_decide (sender candidateTx <> addr)
+              then (balanceLb sres)
+              else (balanceLb sres - maxTxFee)) `min` configuredRB sres)
+      else if bool_decide (sender candidateTx <> addr)
+           then preCandidateTxRes addr
+           else notdelegated
+                  (* because [balanceLb] is just a lowerbound and not exact, we cannot determine whether the tx will revert thus we need to subtract [value candidateTx] unconditionally. EVM execution is not monotone *)
+                  {| balanceLb := balanceLb sres - value candidateTx - maxTxFee;
+                    configuredRB := configuredRB sres;
+                    feeSolvent := feeSolvent sres
+                                  && bool_decide (maxTxFee <= balanceLb sres)|}
+  end.
 
-Fixpoint remainingEffReserveBalsL (preRestResBalances: EffReserveBals) (postStateAccountedSuffix rest: list TxWithHdr)
+Fixpoint remainingEffReserveBalsL (preRestResBalances: EffReserveBals) (rest: list TxWithHdr)
   : EffReserveBals:=
   match rest with
   | [] => preRestResBalances
   | hrest::tlrest =>
       let remainingReserves :=
-        remainingEffReserveBals preRestResBalances postStateAccountedSuffix hrest in
-      remainingEffReserveBalsL remainingReserves (postStateAccountedSuffix++[hrest]) tlrest
+        remainingEffReserveBals preRestResBalances hrest in
+      remainingEffReserveBalsL remainingReserves tlrest
   end.
 
 (** ** Algorithm 1 (consensus): acceptability of a suffix
@@ -301,7 +307,7 @@ Definition consensusAcceptableTxs (latestState : AugmentedState) (proposedTxs: l
   forall addr,
     addr ∈ map sender proposedTxs
     -> match remainingEffReserveBalsL
-               (initialEffReserveBals latestState) [] proposedTxs addr with
+               (initialEffReserveBals latestState) proposedTxs addr with
        | delegated erb => 0 <= erb                                                                     | notdelegated res => feeSolvent res = true
        end.
 
@@ -396,6 +402,7 @@ Definition execValidatedTx  (s: AugmentedState) (t: TxWithHdr)
        then true
        else
          if bool_decide (sender t =a)
+         (* TODO: figure out what breaks if [isAllowedToEmptyExec] is changed to addrDelegated s (sender t) || (sender t) ∈ dels t *)
          then if isAllowedToEmptyExec s t then true else bool_decide ((erb  - maxTxFee t) <= balanceOfAc si a)
          else bool_decide (erb <= balanceOfAc si a) in
      let allBalCheck : bool := (forallb balCheck changedAccounts) in (* in impl, only do for updates *)
@@ -1125,12 +1132,12 @@ Hint Rewrite @updateKeyLkp3 : syntactic.
 
 Definition sresLe (rb1 rb2: ShallowExecRes) :=
   match rb1, rb2 with
-  | notdelegated (mkNotDelCase balLb crb fs), notdelegated (mkNotDelCase balLb2 crb2 fs2)
-    => balLb <= balLb2 /\ crb = crb2 /\ (implb fs fs2)
-  | delegated erb, notdelegated (mkNotDelCase balLb crb _)
-    => (balLb `min` crb) <= erb
+  | notdelegated res1, notdelegated res2
+    => balanceLb res1 <= balanceLb res2
+       /\ configuredRB res1 = configuredRB res2
+       /\ (feeSolvent res1 = true -> feeSolvent res2 = true)
   | delegated erb, delegated erb2 => erb <= erb2
-  | notdelegated _, delegated _ => False
+  | _, _ => False
   end.
 
 Notation "l '`resLe`' r" := (sresLe l r) (at level 50).
@@ -1146,32 +1153,49 @@ Definition rbLe (eoas: list EvmAddr) (rb1 rb2: EffReserveBals) :=
 
  *)
 
-(* this lemma was never needed anyway 
-Lemma mono eoas s rb1 rb2 inter tx:
+Lemma rbLeImpl a b :
+  a `resLe` b ->
+  match a with
+  | delegated erb => 0 ≤ erb
+  | notdelegated res => feeSolvent res = true
+  end ->
+  match b with
+  | delegated erb => 0 ≤ erb
+  | notdelegated res => feeSolvent res = true
+  end.
+Proof.
+  intros Hr.
+  hnf in Hr.
+  destruct a, b; simpl in *; try lia; try case_match; try tauto.
+Qed.
+Ltac sauto := simpl in *; autorewrite with syntactic in *; try lia; try congruence; try eauto.
+
+Lemma mono eoas rb1 rb2 tx:
   rbLe eoas rb1 rb2
-  -> rbLe eoas (remainingEffReserveBals s rb1 inter tx)
-       (remainingEffReserveBals s rb2 inter tx).
+  -> rbLe eoas (remainingEffReserveBals rb1 tx)
+       (remainingEffReserveBals rb2 tx).
 Proof using.
   intros Hrb addr Hin.
   unfold remainingEffReserveBals.
-  pose proof (Hrb addr Hin).
-  case_match_concl; auto;
-    repeat rewrite updateKeyLkp3;
-    fold EffReserveBals in *.
-  {case_bool_decide; subst; try lia.  case_match_concl; auto; simpl in *; try lia. }
-  case_match_concl;
-    repeat rewrite updateKeyLkp3;
-    fold EffReserveBals in *.
-  2:{ case_bool_decide; subst; simpl in *; try lia.  }
-  case_bool_decide;
-    repeat rewrite updateKeyLkp3;
-    fold EffReserveBals in *.
-  2:{ case_bool_decide; subst; try lia. }
-  case_bool_decide;
-    repeat rewrite updateKeyLkp3;
-    fold EffReserveBals in *; try lia.
+  pose proof (Hrb addr Hin) as Hrba.
+  unfold sresLe in Hrba.
+  case_match_concl; auto; rdestruct (rb2 addr); sauto.
+  { (* rb1 and rb2 are delegated *)
+    simpl.
+    case_bool_decide; auto.
+    case_match; try lia.
+  }
+  {
+    case_bool_decide; case_bool_decide; try sauto.
+    forward_reason.
+    autorewrite with iff.
+    split_and !; try sauto.
+    intros.
+    forward_reason.
+    rwHyps.
+    lia.
+  }
 Qed.
- *)
 
 (** In the proof of the main correctness theorem, we use a slightly different
 variant of monotoncity, where in the RHS of [<=], remainingEffReserveBals starts
@@ -1180,7 +1204,6 @@ is dropped from the list of intermediate transactions between the state
 and the candidate transaction [txc].
 The proof follows from the definition of [remainingEffReserveBals]
 and the execution lemmas above.
-*)
 Lemma mono2 tx txc extension s (eoas: list EvmAddr) (rb1 rb2: EffReserveBals) inter:
   (∀ ac : EvmAddr,
       ac ∈ sender tx :: sender txc :: map sender extension
@@ -1225,35 +1248,34 @@ Proof using.
     repeat rewrite updateKeyLkp3;
     fold EffReserveBals in *; simpl in *; try lia.
 Qed.  
+*)
 
 
 (** lifts [mono] from [remainingEffReserveBals] to [remainingEffReserveBalsL]:
 proof follows a straightforward induction on the list [extension],
 using [mono] to fulfil the obligations of the induction hypothesis
  *)
-(* this lemma was never needed anyway 
-Lemma monoL eoas s rb1 rb2 inter extension:
+Lemma monoL eoas rb1 rb2 extension:
   map sender extension ⊆ eoas
   -> rbLe eoas rb1 rb2
-  -> rbLe eoas (remainingEffReserveBalsL s rb1 inter extension)
-          (remainingEffReserveBalsL s rb2 inter extension).
+  -> rbLe eoas (remainingEffReserveBalsL rb1 extension)
+          (remainingEffReserveBalsL rb2 extension).
 Proof using.
-  revert rb1 rb2 inter.
+  revert rb1 rb2.
   induction extension; auto;[].
   unfold rbLe in *.
-  intros ? ? ? Hs Hrb addr Hin. simpl in *.
+  intros ? ?  Hs Hrb addr Hin. simpl in *.
   simpl.
   apply IHextension;[set_solver | | set_solver].
   apply mono.
   assumption.
 Qed.
- *)
 
 (** Similarly, lifts [mono2] from [remainingEffReserveBals] to [remainingEffReserveBalsL]:
 proof follows a straightforward induction on the list [extension],
 using [mono2] to fulfil the obligations of the induction hypothesis.
  *)
-
+(*
 Lemma monoL2 eoas s rb1 rb2 inter extension tx:
   (map sender extension) ⊆ eoas
   -> rbLe eoas rb1 rb2
@@ -1275,9 +1297,42 @@ Proof using.
   clear Hin. clear addr.
   eapply mono2; eauto.
 Qed.
-
+*)
 
 Hint Rewrite initResBal configuredReserveBalOfAddrSpec addrDelegatedUnchangedByBalUpd: syntactic.
+
+Lemma execPreservesConsensusChecks tx extension s:
+  maxTxFee tx <= balanceOfAc s.1 (sender tx) ->
+  (forall txext, txext ∈ extension ->  txBlockNum txext - K ≤ txBlockNum tx ≤ txBlockNum txext)   -> (forall txext, txext ∈ tx::extension ->  txCannotCreateContractAtAddrs txext (map sender (tx::extension)))
+  -> (forall ac, ac ∈ (map sender (tx::extension)) -> hasCode s.1 ac = false)
+  -> consensusAcceptableTxs s (tx::extension)
+  -> consensusAcceptableTxs (execValidatedTx s tx) extension.
+Proof using.
+  intros Hfee Hext Heoac Hsc.
+  clear Hext. execTx
+  pose proof (hasCodeFalsePresExec _ _ _ Heoac Hsc) as Hscf.
+  clear Heoac.
+  set (sf:=(execValidatedTx s tx).1).
+  intros Hc.
+  simpl in *.
+  intros ac Hin.
+  specialize (Hc ac).
+  forward_reason.
+  simpl in *.
+  specialize (Hc ltac:(set_solver)).
+  revert Hc.
+  apply rbLeImpl.
+  pose proof (monoL (map sender (tx::extension))) as Hm.
+  unfold rbLe in Hm.
+  apply Hm; auto; simpl in *; auto; [ set_solver | | set_solver].
+  intros.
+  clear Hm.
+  clear Hc. clear Hin. clear ac.
+  hnf.
+  clear Hsc.
+  clear Hext.
+  apply exec1; auto.
+Qed.
 
 (** This lemma captures a key property of [remainingEffReserveBals]: it underapproximates
 the resultant effective balance after execution of the transaction
@@ -1286,11 +1341,10 @@ Lemma exec1 tx extension s :
   maxTxFee tx <= balanceOfAc s.1 (sender tx)
   -> let sf := (execValidatedTx s tx) in
      (∀ ac : EvmAddr, ac ∈ sender tx :: map sender extension → hasCode sf.1 ac = false)
-     -> (∀ addr : EvmAddr,
-            addr ∈ sender tx :: map sender extension
-            -> let rba := remainingEffReserveBals s (initialEffReserveBals s) [] tx addr in
-               let initEff := initialEffReserveBals sf addr in
-              rba.1 <= initEff.1 /\ rba.2 = initEff.2).
+     -> ∀ addr : EvmAddr,
+         addr ∈ sender tx :: map sender extension
+         -> (remainingEffReserveBals (initialEffReserveBals s) tx addr)
+              `resLe` (initialEffReserveBals sf addr).
 Proof using.
   intros Hfee ? Hscf.
   intros ? Hin.
